Scribblings towards a Hoare-ish logic for register machines.

examples/computability/register/regScript.sml
@@ -176,13 +176,13 @@ val Halts_def =
 (* The function computed by program prog is given by funOf prog.             *)
 (*---------------------------------------------------------------------------*)
 
-val funOf_def =
- Define
-  `funOf prog args =
-     let seq = execOf prog 1 args
+val funOf_def = Define `
+  funOf prog args =
+     let seq = execOf prog 1 (0::args)
      in case haltsAt prog seq of
           SOME m => SOME (reg0 (seq m))
-        | NONE => NONE`;
+        | NONE => NONE
+`;
 
 (*---------------------------------------------------------------------------*)
 (* Accept/reject inputs.                                                     *)
@@ -228,23 +228,345 @@ val IN_Computable = Q.prove
 
 val Run_def =
  Define
-  `Run prog args n = FUNPOW (Step prog) n <| regs := fmapOf args; pc := 1|>`;
+  `Run prog args n =
+     FUNPOW (Step prog) n <| regs := fmapOf (0::args); pc := 1|>`;
+
+val whileRun_def = Define`
+  whileRun prog args =
+    WHILE (λc. ¬haltedConfig prog c) (Step prog)
+          <| regs := fmapOf (0::args); pc := 1 |>
+`
 
 (*---------------------------------------------------------------------------*)
 (* Example Register program executions.                                      *)
 (*---------------------------------------------------------------------------*)
 
+val predOf_def = Define`
+  predOf P s <=> P s.pc (saferead s.regs)
+`
+
+val firstHaltsAt_def = Define`
+  firstHaltsAt prog n s <=>
+    haltedConfig prog (FUNPOW (Step prog) n s) ∧
+    ∀m. m < n ⇒ ¬haltedConfig prog (FUNPOW (Step prog) m s)
+`;
+
+val HOARE_def = Define`
+  HOARE P prog Q <=>
+    ∀s0. predOf P s0 ⇒
+         ∃n. firstHaltsAt prog n s0 ∧
+             predOf Q (FUNPOW (Step prog) n s0)
+`
+
+
+val RPmove_def = Define`
+  RPmove src dest basei exiti =
+    FEMPTY |+ (basei, TST src exiti (basei + 1))
+           |+ (basei + 1, INC dest basei)
+`
+
+val saferead_update = store_thm(
+  "saferead_update",
+  ``((fm |+ (k1,v)) '' k1 = v) ∧
+    (k1 ≠ k2 ⇒ ((fm |+ (k1,v)) '' k2 = fm '' k2))``,
+  SRW_TAC [][saferead_def, FLOOKUP_UPDATE]);
+
+val _ = overload_on("RM*", ``λp n s. FUNPOW (Step p) n s``)
+open lcsymtacs
+val haltedConfig_suffix = store_thm(
+  "haltedConfig_suffix",
+  ``haltedConfig p (RM* p m s) ∧ m ≤ n ⇒ haltedConfig p (RM* p n s)``,
+  Induct_on `n` >| [
+    strip_tac >> `m = 0` by decide_tac >> fsrw_tac [][],
+    Cases_on `m = SUC n` >- srw_tac [][] >>
+    strip_tac >> `m ≤ n` by decide_tac >>
+    srw_tac [][FUNPOW_SUC] >>
+    `haltedConfig p (RM* p n s)` by METIS_TAC [] >>
+    `(RM* p n s).pc ∉ FDOM p` by METIS_TAC [haltedConfig_def] >>
+    srw_tac [][Step_def, FLOOKUP_DEF]
+  ]);
+
+val firstHaltsAt_prefix = store_thm(
+  "firstHaltsAt_prefix",
+  ``∀m n plus_mn s0.
+       firstHaltsAt prog n (FUNPOW (Step prog) m s0) ∧
+       ¬haltedConfig prog (FUNPOW (Step prog)m s0) ∧ (plus_mn = m + n) ⇒
+       firstHaltsAt prog (plus_mn) s0``,
+  SIMP_TAC (srw_ss()) [firstHaltsAt_def] THEN SRW_TAC [][] THENL [
+    FULL_SIMP_TAC (srw_ss() ++ ARITH_ss) [GSYM FUNPOW_ADD],
+    Cases_on `m' ≤ m` >- METIS_TAC [haltedConfig_suffix] >>
+    `m < m'` by decide_tac >>
+    first_x_assum (qspec_then `m' - m` mp_tac) >>
+    srw_tac [ARITH_ss][GSYM FUNPOW_ADD]
+  ]);
+
+val move_correct = store_thm(
+  "move_correct",
+  ``exiti ≠ basei ∧ exiti ≠ basei + 1 ∧ src ≠ dest ∧
+    (∀pc regs. P pc regs ⇒
+               (pc = basei) ∧
+               Q exiti ((src =+ 0) ((dest =+ regs src + regs dest) regs))) ⇒
+    HOARE P (RPmove src dest basei exiti) Q``,
+  SRW_TAC [][RPmove_def, HOARE_def, predOf_def] THEN RES_TAC THEN
+  Q.EXISTS_TAC `2 * s0.regs '' src + 1` THEN
+  Q.PAT_ASSUM `Q XX YY` MP_TAC THEN
+  Q.PAT_ASSUM `s0.pc = basei` MP_TAC THEN
+  Q.ABBREV_TAC `n = s0.regs '' src` THEN
+  POP_ASSUM (MP_TAC o REWRITE_RULE [markerTheory.Abbrev_def]) THEN
+  Q.PAT_ASSUM `P XX YY` (K ALL_TAC) THEN
+  MAP_EVERY Q.ID_SPEC_TAC [`s0`, `n`] THEN Induct THENL [
+    REPEAT GEN_TAC THEN DISCH_THEN (ASSUME_TAC o SYM) THEN
+    REPEAT (DISCH_THEN STRIP_ASSUME_TAC) THEN
+    SIMP_TAC (srw_ss()) [] THEN
+    Q.MATCH_ABBREV_TAC `firstHaltsAt prog 1 s0 ∧ QQ` THEN
+    Q.RM_ABBREV_TAC `QQ` THEN
+    Q.MATCH_ABBREV_TAC `firstHaltsAt prog 1 s0 ∧ Q s.pc ($'' s.regs)` THEN
+    `s = s0 with pc := exiti`
+       by (ASM_SIMP_TAC (srw_ss()) [Step_def, Abbr`s`, Abbr`prog`] THEN
+           ASM_SIMP_TAC (srw_ss()) [FLOOKUP_UPDATE]) THEN
+    SRW_TAC [][] THENL [
+      SRW_TAC [][Abbr`prog`, firstHaltsAt_def, haltedConfig_def,
+                 DECIDE ``∀x. x < 1 ⇔ (x = 0)``],
+      Q.PAT_ASSUM `Q PP SS` MP_TAC THEN
+      Q.MATCH_ABBREV_TAC `Q exiti fm1 ==> Q exiti fm2` THEN
+      Q_TAC SUFF_TAC `fm1 = fm2` THEN1 SRW_TAC [][] THEN
+      SRW_TAC [][Abbr`fm1`, Abbr`fm2`, FUN_EQ_THM,
+                 combinTheory.APPLY_UPDATE_THM] THEN
+      SRW_TAC [][] THEN SRW_TAC [][]
+    ],
+    GEN_TAC THEN DISCH_THEN (ASSUME_TAC o SYM) THEN
+    REPEAT (DISCH_THEN STRIP_ASSUME_TAC) THEN
+    Q.MATCH_ABBREV_TAC `firstHaltsAt prog m s0 ∧ QQ` THEN
+    Q.RM_ABBREV_TAC `QQ` THEN
+    Q.MATCH_ABBREV_TAC `firstHaltsAt prog m s0 ∧ Q s.pc ($'' s.regs)` THEN
+    `s = FUNPOW (Step prog) (2 * n + 1) (FUNPOW (Step prog) 2 s0)`
+      by SRW_TAC [ARITH_ss][Abbr`s`, Abbr`m`, MULT_CLAUSES,
+                            GSYM FUNPOW_ADD] THEN
+    Q.ABBREV_TAC `s1 = FUNPOW (Step prog) 2 s0` THEN
+    `s1 = <| pc := basei;
+             regs := s0.regs |+ (src,n) |+ (dest,s0.regs '' dest + 1) |>`
+       by (RES_TAC THEN
+           SRW_TAC [][Abbr`s1`, Step_def, numeralTheory.numeral_funpow,
+                      Abbr`prog`, FLOOKUP_UPDATE] THEN
+           SRW_TAC [][theorem "config_component_equality",
+                      saferead_update]) THEN
+    FIRST_X_ASSUM (Q.SPEC_THEN `s1` MP_TAC) THEN
+    ASM_SIMP_TAC (srw_ss()) [saferead_update] THEN
+    Q.MATCH_ABBREV_TAC `
+      (Q exiti f ==> firstHaltsAt prog (2 * n + 1) s1' ∧
+                     Q s'.pc ($'' s'.regs)) ⇒
+      firstHaltsAt prog m s0 ∧ Q s'.pc ($'' s'.regs)
+    ` THEN
+    `Q exiti f`
+       by (Q.PAT_ASSUM `Q exiti f0` MP_TAC THEN
+           Q.MATCH_ABBREV_TAC `Q exiti f0 ⇒ Q exiti f` THEN
+           Q_TAC SUFF_TAC `f0 = f` THEN SRW_TAC [][] THEN
+           SRW_TAC [][Abbr`f0`, Abbr`f`, saferead_update, FUN_EQ_THM,
+                      combinTheory.APPLY_UPDATE_THM] THEN
+           SRW_TAC [ARITH_ss][]) >>
+    pop_assum (fn th => srw_tac [][th]) >>
+    match_mp_tac firstHaltsAt_prefix >>
+    map_every qexists_tac [`2`, `2 * n + 1`] >>
+    `¬haltedConfig prog (RM* prog 2 s0)`
+      by srw_tac [ARITH_ss][Abbr`s1`, Abbr`prog`, haltedConfig_def] >>
+    srw_tac [ARITH_ss][Abbr`m`]
+  ]);
+
+val firstHaltsAt_ZERO = store_thm(
+  "firstHaltsAt_ZERO",
+  ``firstHaltsAt p 0 s ⇔ haltedConfig p s``,
+  srw_tac [][firstHaltsAt_def]);
+val _ = export_rewrites ["firstHaltsAt_ZERO"]
+
+
+val firstHaltsAt_SUC = store_thm(
+  "firstHaltsAt_SUC",
+  ``firstHaltsAt p (SUC n) s ⇔
+      firstHaltsAt p n (Step p s) ∧ ¬haltedConfig p s``,
+  srw_tac [][firstHaltsAt_def, FUNPOW, EQ_IMP_THM] >| [
+    first_x_assum (qspec_then `SUC m` mp_tac) >>
+    srw_tac [][FUNPOW],
+    first_x_assum (qspec_then `0` mp_tac) >> srw_tac [][],
+    Cases_on `m = 0` >- srw_tac [][] >>
+    `∃m₀. m = SUC m₀` by (Cases_on `m` >> srw_tac [][]) >>
+    fsrw_tac [][FUNPOW]
+  ]);
+
+val firstHaltsAt_ADD = store_thm(
+  "firstHaltsAt_ADD",
+  ``0 < m ⇒ (firstHaltsAt p (m + n) s ⇔ firstHaltsAt p m (RM* p n s))``,
+  srw_tac [][firstHaltsAt_def, EQ_IMP_THM, FUNPOW_ADD] >| [
+    first_x_assum (qspec_then `m' + n` mp_tac) >>
+    srw_tac [][FUNPOW_ADD],
+    Cases_on `n ≤ m'` >-
+      (first_x_assum (qspec_then `m' - n` mp_tac) >>
+       srw_tac [ARITH_ss][GSYM FUNPOW_ADD]) >>
+    first_x_assum (qspec_then `0` mp_tac) >>
+    srw_tac [][] >>
+    `m' ≤ n` by DECIDE_TAC >>
+    metis_tac [haltedConfig_suffix]
+  ]);
+
+val unused_instructions = store_thm(
+  "unused_instructions",
+  ``∀n m s.
+      firstHaltsAt prog₁ n s ∧ DISJOINT (FDOM prog₁) (FDOM prog₂) ∧ m ≤ n ⇒
+      (RM* (FUNION prog₁ prog₂) m s = RM* prog₁ m s)``,
+  Induct_on `n` >- srw_tac [][] >>
+  srw_tac [][firstHaltsAt_SUC] >>
+  `(m = 0) ∨ ∃m₀. m = SUC m₀` by (Cases_on `m` >> srw_tac [][])
+     >- srw_tac [][] >>
+  `m₀ ≤ n` by fsrw_tac [][] >>
+  `s.pc ∈ FDOM prog₁` by fsrw_tac [][haltedConfig_def] >>
+  `s.pc ∉ FDOM prog₂`
+    by (fsrw_tac [][DISJOINT_DEF, EXTENSION] >> metis_tac []) >>
+  srw_tac [][FUNPOW] >>
+  `Step (FUNION prog₁ prog₂) s = Step prog₁ s`
+    by srw_tac [][Step_def, FLOOKUP_DEF, FUNION_DEF] >>
+  srw_tac [][]);
+
+val haltedConfig_bigger_prog = store_thm(
+  "haltedConfig_bigger_prog",
+  ``haltedConfig (FUNION p₁ p₂) s ⇒ haltedConfig p₁ s``,
+  srw_tac [][haltedConfig_def, FUNION_DEF]);
+
+val predOf_AND_def = Define`
+  predOf_AND p q pc rf ⇔ p pc rf ∧ q pc rf
+`;
+
+val _ = set_fixity "&&" (Infixr 400)
+val _ = overload_on("&&", ``predOf_AND``)
+
+val PCNOTIN_def = Define`
+  PCNOTIN s pc rf ⇔ pc ∉ s
+`
+val _ = overload_on("PC∉", ``PCNOTIN``)
+
+val predOf_AND_thm = store_thm(
+  "predOf_AND_thm",
+  ``predOf (P && Q) s ⇔ predOf P s ∧ predOf Q s``,
+  srw_tac [][predOf_AND_def, predOf_def])
+
+val predOf_PCNOTIN = store_thm(
+  "predOf_PCNOTIN",
+  ``predOf (PC∉ s) c ⇔ c.pc ∉ s``,
+  srw_tac [][PCNOTIN_def, predOf_def]);
+
+val HOARE_sequence = store_thm(
+  "HOARE_sequence",
+  ``HOARE P prog1 R ∧ HOARE R prog2 (Q && PC∉ (FDOM prog1)) ∧
+    DISJOINT (FDOM prog1) (FDOM prog2) ⇒
+    HOARE P (FUNION prog1 prog2) Q``,
+  SRW_TAC [][HOARE_def] THEN
+  `∃n₁. firstHaltsAt prog1 n₁ s0 ∧ predOf R (RM* prog1 n₁ s0)`
+    by METIS_TAC [] THEN
+  Q.ABBREV_TAC `s1 = RM* prog1 n₁ s0` THEN
+  `∃n₂. firstHaltsAt prog2 n₂ s1 ∧
+        predOf (Q && PC∉(FDOM prog1)) (RM* prog2 n₂ s1)`
+    by METIS_TAC [] THEN
+  Q.EXISTS_TAC `n₂ + n₁` THEN ASM_SIMP_TAC (srw_ss()) [FUNPOW_ADD] THEN
+  `∀m. m ≤ n₁ ⇒ (RM* (FUNION prog1 prog2) m s0 = RM* prog1 m s0)`
+    by metis_tac[unused_instructions] >>
+  asm_simp_tac (srw_ss()) [] >>
+  Cases_on `n₂ = 0` >-
+    (fsrw_tac [][firstHaltsAt_def, predOf_AND_thm] >> conj_tac >-
+       fsrw_tac [][haltedConfig_def, FUNION_DEF] >>
+     srw_tac [ARITH_ss][] >> metis_tac [haltedConfig_bigger_prog]) >>
+  `0 < n₂` by decide_tac >>
+  asm_simp_tac (srw_ss()) [firstHaltsAt_ADD] >>
+  `FUNION prog1 prog2 = FUNION prog2 prog1`
+     by metis_tac [FUNION_COMM] >>
+  pop_assum SUBST_ALL_TAC >>
+  `∀m. m ≤ n₂ ⇒ (RM* (FUNION prog2 prog1) m s1 = RM* prog2 m s1)`
+     by metis_tac [DISJOINT_SYM, unused_instructions] >>
+  REVERSE conj_tac >- fsrw_tac [][predOf_AND_thm] >>
+  fsrw_tac [][firstHaltsAt_def] >> conj_tac >-
+    fsrw_tac [][haltedConfig_def, predOf_PCNOTIN, predOf_AND_thm,
+                FUNION_DEF] >>
+  srw_tac [ARITH_ss][] >> metis_tac [haltedConfig_bigger_prog]);
+
 (*
 (* Halt immediately *)
 val prog1 = ``FEMPTY |++ [(1,TST 0 0 0)]``;
 
-(* Add R0 and R1, leaving result in R0 and trashing R1 *)
-val prog2 = ``FEMPTY |++ [(1,TST 1 0 2); (2, INC 0 1)]``;
+(* Add R1 and R2, putting result in R0 and trashing R1 *)
+val prog2 = ``FUNION (RPmove 1 0 1 3) (RPmove 2 0 3 0)``
 
 EVAL ``reg0(Run ^prog1 [0;1;2] 1)``;
 EVAL ``reg0(Run ^prog2 [3;4] 8)``;
 EVAL ``reg0(Run ^prog2 [3;19] 40)``;
 Count.apply EVAL ``reg0(Run ^prog2 [19;52] 400)``;
+
+Count.apply EVAL ``reg0 (whileRun ^prog2 [19;52])``;
+
+val zero_nb1 = prove(
+  ``~(0 = NUMERAL (BIT1 n))``,
+  REWRITE_TAC [NUMERAL_DEF, BIT1, ADD_CLAUSES, SUC_NOT]);
+val nb12 = prove(
+  ``NUMERAL (BIT1 n) <> NUMERAL (BIT2 m)``,
+  REWRITE_TAC [NUMERAL_DEF, BIT1, BIT2, ADD_CLAUSES, SUC_NOT,
+               prim_recTheory.INV_SUC_EQ] THEN
+  DISCH_THEN (MP_TAC o AP_TERM ``EVEN``) THEN
+  SRW_TAC [][EVEN_ADD, EVEN]);
+
+val keycollapse1 = prove(
+  ``fm |+ (0, v1) |+ (NUMERAL (BIT1 n), v2) |+ (0, v3) =
+    fm |+ (0, v3) |+ (NUMERAL (BIT1 n), v2)``,
+  SRW_TAC [][fmap_EXT, EXTENSION, FAPPLY_FUPDATE_THM, zero_nb1] THEN1
+    PROVE_TAC [] THEN
+  SRW_TAC [][] THEN
+  FULL_SIMP_TAC (srw_ss()) [zero_nb1]);
+
+val keycollapse2 = prove(
+  ``fm |+ (NUMERAL (BIT1 n), v1) |+ (NUMERAL (BIT2 m), v2)
+       |+ (NUMERAL (BIT1 n), v3) =
+    fm |+ (NUMERAL (BIT1 n), v3) |+ (NUMERAL (BIT2 m), v2)``,
+  SRW_TAC [][fmap_EXT, EXTENSION, FAPPLY_FUPDATE_THM, nb12] THEN1
+    PROVE_TAC [] THEN
+  SRW_TAC [][] THEN
+  FULL_SIMP_TAC (srw_ss()) [nb12]);
+
+SIMP_CONV (srw_ss()) [Run_def, FUNION_DEF, numeralTheory.numeral_funpow, Step_def, FLOOKUP_FUNION, RPmove_def, FLOOKUP_UPDATE, fmapOf_def, saferead_def, FUPDATE_LIST_THM, keycollapse1, keycollapse2] ``Run ^prog2 [19;52] 41``
+
 *)
 
+(* Implementations of the recursive functions *)
+(* results put into register 0; arguments in registers 1 .. n *)
+
+val zeroRP_def = Define`
+  zeroRP zr bi ei = FEMPTY |+ (bi,TST zr ei bi)
+`;
+
+(* val zeroRP_correct = store_thm(
+  "zeroRP_correct",
+  ``bi ≠ ei ∧ (∀pc r. P pc r ⇒ (pc = bi) ∧ Q ei ((zr =+ 0) r)) ⇒
+    HOARE P (zeroRP zr bi ei) Q``,
+  srw_tac [][HOARE_def] >>
+  qexists_tac `s0.regs '' zr + 1` >>
+  fsrw_tac [][predOf_def] >> res_tac >>
+  ntac 2 (pop_assum mp_tac) >>
+  qabbrev_tac `n = s0.regs '' zr` >>
+  pop_assum (mp_tac o REWRITE_RULE [markerTheory.Abbrev_def]) >>
+  pop_assum (K ALL_TAC) >>
+  map_every qid_spec_tac [`s0`, `n`] >> Induct >| [
+    gen_tac >> disch_then (assume_tac o SYM) >>
+    srw_tac [][firstHaltsAt_def, Step_def, zeroRP_def, FLOOKUP_UPDATE,
+               haltedConfig_def, DECIDE ``x < 1 ⇔ (x = 0)``] >>
+    pop_assum mp_tac >>
+    qmatch_abbrev_tac `Q ei f1 ==> Q ei f2` >>
+    `f1 = f2`
+       by (srw_tac [][FUN_EQ_THM, combinTheory.APPLY_UPDATE_THM, Abbr`f1`,
+                      Abbr`f2`] >>
+           srw_tac [][] >> srw_tac [][]) >>
+    srw_tac [][],
+    gen_tac >> disch_then (assume_tac o SYM) >>
+    asm_simp_tac (srw_ss()) [ADD_CLAUSES, firstHaltsAt_SUC, FUNPOW] >>
+    rpt (disch_then strip_assume_tac) >>
+    `¬haltedConfig (zeroRP zr bi ei) s0`
+       by srw_tac [][haltedConfig_def, zeroRP_def] >>
+    asm_simp_tac (srw_ss()) [] >>
+    RULE_ASSUM_TAC (PURE_REWRITE_RULE [AND_IMP_INTRO]) >>
+    first_x_assum match_mp_tac >>
+    `Step (zeroRP zr bi ei) s0 = <| pc := bi; regs := s0.regs |+ (zr, s0.regs '' zr - 1)|>`
+*)
 val _ = export_theory();
